theories/deciderel/examples.v
@@ -1,0 +1,50 @@
+From MetaCoq.Template Require Import utils All.
+Unset MetaCoq Strict Unquote Universe Mode.
+From SMTCoq Require Import SMTCoq.
+Import MCMonadNotation.
+Require Import List.
+Import ListNotations.
+Require Import String.
+Require Import ZArith.
+Require Import Bool.
+Require Import proof_correctness.
+
+(* A first example :
+mem n l is true whenever n belongs to l 
+the plugin linearize the type of MemMatch because n is mentionned twice 
+so we have an equivalent version linearized of member and then it generates an 
+equivalent boolean fixpoint and the correctness lemma
+*) 
+
+(* Need to convert ltac2 tactic within ltac1 for compatibility reasons with MetaCoq *)
+Tactic Notation "correctness" constr(t) constr(t') constr(n) constr(n') := 
+let tac := 
+ltac2:(t1 t2 n n' |- let t1' := ltac1_to_constr_unsafe t1 in
+                  let t2' := ltac1_to_constr_unsafe t2 in
+                  let n0 := constr_to_int (ltac1_to_constr_unsafe n) in
+                  let n0' := constr_to_int (ltac1_to_constr_unsafe n') in correctness_auto t1' t2' n0 n0') in 
+timeout 5 (tac t t' n n').
+
+Ltac correctness_ltac1 t t' n n' := correctness t t' n n'.
+
+Inductive mem : nat -> list nat -> Prop :=
+    MemMatch : forall (xs : list nat) (n : nat), mem n (n :: xs)
+  | MemRecur : forall (xs : list nat) (n n' : nat), mem n xs -> mem n (n' :: xs).
+
+MetaCoq Run (decide mem []). 
+Next Obligation.
+(* the proof can be partially automatized thanks to tactics :
+completeness_auto_npars takes the name of the fixpoint generated and the number of parameters 
+as input and tries to generate the proof automatically 
+soundness_auto_recarg_npars takes the name of the initial inductive, the argument 
+on which to recur and the number of parameters of the inductive *)
+- revert_all. ltac2:(completeness_auto_npars 'mem_linear_decidable 0).
+- revert_all. ltac2:(soundness_auto_recarg_npars 'mem_linear_decidable 1 0). Defined.
+
+
+
+
+
+ 
+
+
